# 复合函数求导训练

<hr>

#First

$$y=tan\frac{2x}{1+x^{2}},\quad y'=?$$
$$\\ \\$$

$$
y=tanu,
u=\frac{2x}{1+x^{2}},\quad
y'=(tanu)'(u)'
$$

$$\\ \\$$
$$(tanu)'=sec^{2}\frac{2x}{1+x^{2}}$$
$$\\ \\$$
$$(u)'=\frac{(2x)'(1+x^{2})-(1+x^{2})2x}{(1+x^{2})^{2}}$$
$$\\ \\$$

$$
(2x)'=2,\\
(1+x^{2})'=(1)'+(x^{2})'=0+2x=2x
$$

$$\\ \\$$
$$\therefore (u)'=\frac{2(1+x^{2})-2x \cdot 2x}{(1+x^{2})^{2}}=\frac{2-2x^{2}}{(1+x^{2})^{2}}$$
$$\\ \\$$
$$y'=(tanu)'(u)'=sec^{2}\frac{2x}{1+x^{2}} \cdot \frac{2-2x^{2}}{(1+x^{2})^{2}}$$

<hr>

#Second

$$
y=ln(3x^{2}+x+1),\quad
y'=?
$$

$$\\ \\$$

$$
y=lnu,\quad
u=3x^{2}+x+1,\\
\therefore y'=(lnu)'(u)'
$$

$$\\ \\$$
$$(u)'=(3x^{2})'+(x)'+(1)'=(6x+1)+0+0$$
$$\\ \\$$
$$(lnu)'=\frac{1}{ulne}=\frac{1}{u}=\frac{1}{3x^{2}+x+1}$$
$$\\ \\$$
$$\therefore y'=\frac{6x+1}{3x^{2}+x+1}$$

<hr>

#Third

$$f(x)=(1+sinx)^{2},\quad f'(x)=?$$
$$\\ \\$$

$$
设u(x)=1+sinx,\quad
则f(u)=u^{2}\\
f'(x)=f'[u(x)]=f'(u)\cdot u'(x)
$$

$$\\ \\$$
$$f'(u)=(u^{2})'=2u=2(1+sinx)$$
$$\\ \\$$
$$u'(x)=(1+sinx)'=cosx$$
$$\\ \\$$
$$\therefore f'(x)=f'[u(x)]=2(1+sinx)cosx$$

<hr>
  
  
#Fourth

$$y=cos\sqrt[]{1+lnx},\quad y'=?$$
$$\\ \\$$

$$
设u=\sqrt[]{1+lnx},则y(u)=cosu
\\
$$

$$
\\
设\alpha =1+lnx,  则\alpha(x)=1+lnx, \quad u(\alpha)=\sqrt[]{\alpha}
$$

$$\\ \\$$

$$
y'=y'(x)=y'\{ u[\alpha (x)] \}=y'(u)\cdot u'(\alpha )\cdot \alpha' (x)
$$

$$\\ \\$$
$$y'(u) =(cosu)'=-sinu$$
$$\\ \\$$
$$u'(\alpha )=(\sqrt[]{\alpha })'=\frac{1}{2\sqrt[]{\alpha } } $$
$$\\ \\$$
$$\alpha' (x)=(1+lnx)'=\frac{1}{x} $$
$$\\ \\$$

$$
\frac{1}{x} \cdot \frac{1}{2\sqrt[]{\alpha}} \cdot -sinu=
\frac{-sin\sqrt[]{1+lnx} }{2x\sqrt[]{1+lnx} }
$$

$$\\ \\$$

$$
y'=\frac{-sin\sqrt[]{1+lnx} }{2x\sqrt[]{1+lnx} }
$$

<hr>
  
# Fifth
$$f'(x)=ln\sqrt[]{1+x^{2}},\quad f'(x)=? $$
$$\\ \\$$
$$
设\beta=1+x^{2}, \quad u=\sqrt[]{1+x^{2}} \\
则\beta(x)=1+x^{2},\quad u(\beta)=\sqrt[]{1+x^{2}},\quad f(u)=lnu$$
$$\\ \\$$
$$
\because f(x)=f'\{ u[\beta(x)]\}\\
\therefore f'(x)=f'\{ u[\beta(x)]\}=f'(u)\cdot u'(\beta) \cdot \beta '(x)$$
$$\\ \\$$
$$
f'(u)=\frac{1}{u}
\\
u'(\beta) =\frac{1}{2\sqrt[]{\beta} } 
\\
\beta '(x)=2x
$$
$$\\ \\$$
$$
\frac{1}{u} \cdot \frac{1}{2\sqrt[]{\beta} } \cdot 2x
=\frac{1}{\sqrt[]{1+x^{2}} } \cdot \frac{1}{2\sqrt[]{1+x^{2}} } \cdot 2x
=\frac{x}{1+x^{2}} 
$$
$$\\ \\$$
$$\therefore f'(x)=\frac{x}{1+x^{2}} $$  
  
  
  
#Sixth
  
**本题采用了对数求导法**  
  


$$y = \sqrt[4]{ \frac{(x-1)(x-2)}{(x-3)(x-4)} },\quad y'(x)=?$$

$$\\ \\ $$
$$y=[\frac{(x-1)(x-2)}{(x-3)(x-4)}]^{\frac{1}{4}}$$
$$\\ \\ $$

$$\\ \\ $$
$$\log{ \frac{(x-1)(x-2)}{(x-3)(x-4)} } {y}=\frac{lny}{ln\frac{(x-1)(x-2)}{(x-3)(x-4)}}=\frac{1}{4}$$
$$\\ \\ $$
$$lny=\frac{1}{4} ln[\frac{(x-1)(x-2)}{(x-3)(x-4)}]$$
$$\\ \\ $$
$$lny =\frac{1}{4} [ln(x-1)+ln(x-2)-ln(x-3)-ln(x-4)] $$
$$\\ \\ $$

同时对两边求导(注意系数 $\frac{1}{4}$ 不纳入求导范围内):

$$\frac{d(lny)}{dx} \cdot \frac{dy}{dx}=\frac{1}{4} \frac{d[ln(x-1)+ln(x-2)-ln(x-3)-ln(x-4)]}{dx}$$
$$\\ \\ $$
$$\frac{1}{y}\cdot \frac{dy}{dx}=\frac{1}{4} [\frac{1}{x-1}+\frac{1}{x-2}-\frac{1}{x-3}-\frac{1}{x-4}] $$
$$\\ \\ $$
$$\frac{dy}{dx}=\frac{1}{4} [\frac{1}{x-1}+\frac{1}{x-2}-\frac{1}{x-3}-\frac{1}{x-4}] \cdot y$$
$$\\ \\ $$

$$
\frac{dy}{dx}=\frac{1}{4} [\frac{1}{x-1}+\frac{1}{x-2}-\frac{1}{x-3}-\frac{1}{x-4}] \cdot \sqrt[4]{ \frac{(x-1)(x-2)}{(x-3)(x-4)} }
$$

$$\\ \\ $$
$$\therefore y'(x)=\frac{1}{4} [\frac{1}{x-1}+\frac{1}{x-2}-\frac{1}{x-3}-\frac{1}{x-4}] \cdot \sqrt[4]{ \frac{(x-1)(x-2)}{(x-3)(x-4)} }$$
