# 韦达定理之推导

<hr>

$$ax^2+bx+c = 0 $$
$$\\ \\$$
$$a(x^2+\frac{b}{a}x+\frac{c}{a}) = 0$$

$$\\ \\$$
$$x^2+\frac{b}{a}x = -\frac{c}{a}  $$

$$\\ \\$$
$$x^2+\frac{b}{a}x+(\frac{b}{2a})^2 = -\frac{c}{a}+(\frac{b}{2a})^2$$

$$\\ \\$$
$$(x+\frac{b}{2a})^2 = \frac{b^2-4ac}{4a^2} $$

$$\\ \\$$ 

$$x_{1} = \frac{\sqrt[]{b^2-4ac}-b}{2a} $$

$$\\ \\$$
$$x_{2} = \frac{-\sqrt[]{b^2-4ac}-b}{2a} $$
$$\\ \\$$
$$设b^2-4ac=\Delta$$
$$\\ \\$$
$$\because x_{1}=\frac{ \sqrt[]{\Delta}-b}{2a} $$
$$\\ \\$$
$$\because x_{2}=\frac{ -\sqrt[]{\Delta}-b}{2a} $$
$$\\ \\$$
$$\therefore x_{1}+x_{2}=-\frac{b}{a}$$
$$\\ \\$$ 
$$\therefore x_{1} \cdot x_{2}=\frac{c}{a} $$
