# 导数乘法和除法公式证明

<hr>

# 乘法

$$若f( x)g( x)= h(x),求证h'( x)=f'( x)g( x)+ f( x) g '(x )$$
$$\\ \\$$
$$即证明[f(x)\cdot g(x)] ' = f '(x)g(x)+ f(x)g '(x )$$
$$\\ \\$$

$$
h '(x)= \lim_{ Δx \to 0 } \frac { h(x + Δx)- h(x)} { Δx } =\lim_{ Δx \to 0 }
\frac{ f(x + Δx)g(x + Δx)- f (x)g(x) } { Δx }
$$

$$\\ \\$$

$$
变形:\\
\lim_{ Δx \to 0 }\frac { f(x+ Δx)g(x) - f(x)g(x+Δx) + f(x)g(x+Δx) - f( x)g( x)} { Δx }
$$

$$\\ \\$$

$$\lim_{Δx \to 0} \frac{ g( x+Δx) [ f(x + Δx)- f(x)] } { Δx } + \frac{ f( x)[ g( x +Δx)- g(x)] } { Δx }$$

$$\\ \\$$
$$\lim_{ Δx \to 0 }g(x + Δx)f ' (x) + f(x) g ' (x)$$
$$\\ \\$$
$$\because \lim_{ Δx \to 0 }  Δx =0$$
$$\\ \\$$
$$\therefore \lim_{ Δx \to 0 } g( x + Δx)= g(x)$$
$$\\ \\$$
$$\Rightarrow g(x)f'(x)+  f(x)g'(x)$$
$$\\ \\$$
**证明成立**

<hr>

# 除法

$$证明[\frac{f(x)}{g(x)} ]'=\frac { f'(x) g(x) - f(x) g'(x) } { g^{2}(x)}$$
$$\\ \\$$
$$\lim_{ Δx \to 0 } \frac{ 1 } { Δx }\cdot \frac { f(x+Δx) } { g(x+Δx) } - \frac { f(x) } { g(x) }$$
$$\\ \\$$
$$\frac{1}{Δx}\cdot \frac { f(x+Δx) g(x) } { g(x+Δx) g(x) } - \frac{ f(x) g(x+Δx) } { g(x) g(x+Δx) }$$
$$\\ \\$$
$$\frac{1}{Δx} \cdot \frac { f(x+Δx)g(x) - f(x)g(x+Δx) } { g(x)g(x+Δx) }$$
$$\\ \\$$
$$\frac { f(x+Δx)g(x) - f(x)g(x+Δx) } { Δx } \cdot \frac { 1} { g(x)g(x+Δx) }$$
$$\\ \\$$

$$
参考乘法法则推导过程中的某一步:\\
\lim_{Δx \to 0 } \frac{ f(x+Δx)g(x) - f(x)g(x) + f(x)g(x) - f(x)g(x+Δx) } {Δx} \cdot \frac{ 1 }{g(x)g(x+Δx)}
$$

$$\\ \\$$
$$g(x)\lim_{Δx \to 0 }\frac {f(x+Δx) - f(x) }{Δx } - f(x)\lim_{ Δx \to 0 } \frac { -g(x) + g(x+Δx) }{ Δx }$$
$$\\ \\$$
$$f'( x ) g(x) - f(x) g'( x ) \cdot \lim_{Δx \to 0 } \frac { 1} { g(x)g(x+Δx) }$$
$$\\ \\$$

$$
\because \lim_{ Δx \to 0 } Δx  = 0
\\
\therefore  \lim_{ Δx \to 0 } g(x+Δx)  = g(x)
$$

$$\\ \\$$
$$\therefore =\frac { f'(x) g(x) - f(x) g'(x) } { g(x) \cdot g(x) }$$
$$\\ \\$$
$$=\frac { f'(x) g(x) - f(x) g'(x) } { g^{2}(x)}$$
